updates

Veritas.Blum.fst
@@ -1,6 +1,8 @@
 module Veritas.Blum
 
 open FStar.Seq
+open Veritas.EAC
+open Veritas.Interleave
 open Veritas.MultiSet
 open Veritas.MultiSetHash
 open Veritas.SeqAux
@@ -49,6 +51,21 @@ let rec lemma_hadd_add_set (il:t_verifiable_log):
     | _ -> ()
   )
 
+(* concatenation of all local add-seq *)
+let g_add_seq (gl: g_verifiable_log): seq (ms_hashfn_dom) = 
+  let gl' = g_verifiable_refine gl in
+  (* sequence of local add_sequences *)
+  let l_adds = map add_seq gl' in
+  reduce (Seq.empty #ms_hashfn_dom) append l_adds
+
+(* multiset derived from all the blum adds in gl *)
+let g_add_set (gl: g_verifiable_log): mset ms_hashfn_dom =
+  seq2mset (g_add_seq gl)
+
+(* the hadd that the verifier computes is the multiset hash of all the adds *)
+let lemma_g_hadd_correct (gl: g_verifiable_log):
+  Lemma (g_hadd gl = ms_hashfn (g_add_seq gl)) = admit()
+
 (* sequence of versioned records evicted from a verifier *)
 let rec evict_seq (il:t_verifiable_log):
   Tot (seq ms_hashfn_dom)
@@ -74,6 +91,19 @@ let rec evict_seq (il:t_verifiable_log):
 (* evict multiset of a verifier *)
 let evict_set (il:t_verifiable_log): mset ms_hashfn_dom =
   seq2mset (evict_seq il)
+
+(* a single sequence containing all the blum evicts *)
+let g_evict_seq (gl: g_verifiable_log): seq ms_hashfn_dom = 
+  let gl' = g_verifiable_refine gl in
+  (* sequence of local add_sequences *)
+  let l_evicts = map evict_seq gl' in
+  reduce (Seq.empty #ms_hashfn_dom) append l_evicts 
+
+let g_evict_set (gl: g_verifiable_log): mset ms_hashfn_dom = 
+  seq2mset (g_evict_seq gl)
+
+let lemma_ghevict_correct (gl: g_verifiable_log):
+  Lemma (g_hevict gl = ms_hashfn (g_evict_seq gl)) = admit()
 
 (* the thread id of a verifier remains unchanged *)
 let rec lemma_thread_id (il:t_verifiable_log):
@@ -109,3 +139,59 @@ let rec lemma_hevict_evict_set (il:t_verifiable_log):
       lemma_hashfn_app (evict_seq (id, l')) (MHDom (k,v) t id)
     | _ -> ()
   )
+
+type blum_add_log_entry = e:vlog_entry {AddB? e}
+
+(* sequence of blum adds in a time sequenced log *)
+let ts_add_seq (#n:nat) (itsl: its_log n): seq ms_hashfn_dom =
+  (* all log entries *)
+  let l = project_seq itsl in
+  (* blum add log entries *)
+  let ba: seq blum_add_log_entry = filter_refine AddB? l in
+  map (fun (e:blum_add_log_entry) -> match e with
+                                   | AddB r t j -> MHDom r t j) 
+      ba
+
+(* the addset in a time sequenced log *)
+let ts_add_set (#n:nat) (itsl: its_log n): mset ms_hashfn_dom 
+  = seq2mset (ts_add_seq itsl)
+
+let lemma_ts_add_set_correct (#n:nat) (itsl: its_log n): 
+  Lemma (ts_add_set itsl == g_add_set (partition_idx_seq itsl)) = admit()
+
+let is_blum_evict (#n:nat) (itsl: its_log n) (i: seq_index itsl): bool = 
+  let (e,_) = index itsl i in
+  match e with
+  | EvictB _ _ -> true
+  | EvictBM _ _ _ -> true
+  | _ -> false
+
+let blum_evict_elem (#n:nat) (itsl:its_log n) (i:seq_index itsl{is_blum_evict itsl i}): ms_hashfn_dom = 
+  let (e,id) = index itsl i in
+  let tsle = time_seq_ext itsl in
+  assert(project_seq itsl = to_vlog tsle);
+  lemma_unzip_index itsl i;
+  assert(to_vlog_entry (index tsle i) = e);
+  match e with
+  | EvictB k t -> 
+    let v = Evict?.v (index tsle i) in
+    MHDom (k,v) t id
+  | EvictBM k _ t -> 
+    let v = Evict?.v (index tsle i) in
+    MHDom (k,v) t id
+ 
+let rec ts_evict_seq (#n:nat) (itsl: its_log n): Tot (seq ms_hashfn_dom) 
+  (decreases (length itsl)) =
+  let m = length itsl in 
+  if m = 0 then Seq.empty #ms_hashfn_dom
+  else if is_blum_evict itsl (m - 1) then
+    append1 (ts_evict_seq (its_prefix itsl (m - 1))) (blum_evict_elem itsl (m - 1))   
+  else
+    ts_evict_seq (its_prefix itsl (m - 1))
+
+let ts_evict_set (#n:nat) (itsl: its_log n): mset ms_hashfn_dom = 
+  seq2mset (ts_evict_seq itsl)
+
+let lemma_ts_evict_set_correct (#n:nat) (itsl: its_log n):
+  Lemma (ts_evict_set itsl == g_evict_set (partition_idx_seq itsl)) = admit()
+
