Veritas.MultiSetHash.fsti
@@ -63,17 +63,6 @@ val ms_hashfn_agg (h1: ms_hash_value) (h2: ms_hash_value) : Tot ms_hash_value
 val lemma_hashfn_agg (s1 s2: seq ms_hashfn_dom):
   Lemma (ms_hashfn (append s1 s2) = ms_hashfn_agg (ms_hashfn s1) (ms_hashfn s2))
 
-(* aggregate a sequence of multiset hashes into a single one *)
-val ms_hashfn_agg_seq (hs: seq ms_hash_value): Tot ms_hash_value
-
-(* TODO: Is the correct way to declare this lemma? *)
-val lemma_empty_agg_seq (_:unit) :
-  Lemma (ms_hashfn_agg_seq FStar.Seq.empty = empty_hash_value)
-
-val lemma_app_seq (hs1 hs2: seq ms_hash_value):
-  Lemma (ms_hashfn_agg (ms_hashfn_agg_seq hs1) (ms_hashfn_agg_seq hs2) = 
-         ms_hashfn_agg_seq (append hs1 hs2))
-
 (* multiset hash collision *)
 type ms_hash_collision = 
   | MSCollision: s1: seq ms_hashfn_dom -> 
